Open 'oo_scope' in 'Test.ReduceTactics'
- Instead of always using '%oo' scope delimiter.

He4/Language/Test/ReduceTactics.v
@@ -7,7 +7,6 @@ Require Import He4.Language.Value.
 Require Import He4.Strings.String.
 Require Import He4.Language.ReduceTactics.
 Import ObjectOrientedNotations.
-Delimit Scope oo_scope with oo.
 Import StateNotations.
 
 Notation "t1 '/' st1 '==>' t2 '/' st2" := (step (pair t1 st1) (pair t2 st2))
@@ -17,137 +16,108 @@ Notation "t1 '/' st1 '==>*' t2 '/' st2" := (multi step (pair t1 st1) (pair t2 st
   (at level 40, st1 at level 39, t2 at level 39, format "'//' '[' t1 '//' / '//' st1 '//' '==>*' '//' t2 '//' / '//' st2 ']'").
 
 Section Examples.
+Open Scope oo_scope.
 Open Scope state_scope.
 
-Definition ex_reduce_tnot_tm := ((
-    !!tbool true
-  )%oo).
+Definition ex_reduce_tnot_tm := !!tbool true.
 Example ex_reduce_tnot:
   forall st,
   ex_reduce_tnot_tm / st ==>* tbool true / st.
 Proof.
   unfold ex_reduce_tnot_tm. intros. repeat reduce. Qed.
 
-Definition ex_reduce_tand_tm := ((
-    !tbool false \&& !tbool true \&& tbool true
-  )%oo).
+Definition ex_reduce_tand_tm := !tbool false \&& !tbool true \&& tbool true.
 Example ex_reduce_tand:
   forall st,
   ex_reduce_tand_tm / st ==>* tbool false / st.
 Proof.
   unfold ex_reduce_tand_tm. intros. repeat reduce. Qed.
 
-Definition ex_reduce_tor_tm := ((
-    !tbool true \|| !tbool false \|| tbool false
-  )%oo).
+Definition ex_reduce_tor_tm := !tbool true \|| !tbool false \|| tbool false.
 Example ex_reduce_tor:
   forall st,
   ex_reduce_tor_tm / st ==>* tbool true / st.
 Proof.
   unfold ex_reduce_tor_tm. intros. repeat reduce. Qed.
 
-Definition ex_reduce_tplus_tm := ((
-    (tnat 3 \+ tnat 4) \+ (tnat 5 \+ tnat 6)
-  )%oo).
+Definition ex_reduce_tplus_tm := (tnat 3 \+ tnat 4) \+ (tnat 5 \+ tnat 6).
 Example ex_reduce_tplus:
   forall st,
   ex_reduce_tplus_tm / st ==>* tnat 18 / st.
 Proof.
   unfold ex_reduce_tplus_tm. intros. repeat reduce. Qed.
 
-Definition ex_reduce_tminus_tm := ((
-    (tnat 3 \+ tnat 4) \- (tnat 1 \+ tnat 2)
-  )%oo).
+Definition ex_reduce_tminus_tm := (tnat 3 \+ tnat 4) \- (tnat 1 \+ tnat 2).
 Example ex_reduce_tminus:
   forall st,
   ex_reduce_tminus_tm / st ==>* tnat 4 / st.
 Proof.
   unfold ex_reduce_tminus_tm. intros. repeat reduce. Qed.
 
-Definition ex_reduce_tmult_tm := ((
-    (tnat 3 \+ tnat 4) \* (tnat 1 \+ tnat 2)
-  )%oo).
+Definition ex_reduce_tmult_tm := (tnat 3 \+ tnat 4) \* (tnat 1 \+ tnat 2).
 Example ex_reduce_tmult:
   forall st,
   ex_reduce_tmult_tm / st ==>* tnat 21 / st.
 Proof.
   unfold ex_reduce_tmult_tm. intros. repeat reduce. Qed.
 
-Definition ex_reduce_teq_tm_1 := ((
-    !tbool true \== !tbool false
-  )%oo).
+Definition ex_reduce_teq_tm_1 := !tbool true \== !tbool false.
 Example ex_reduce_teq_1:
   forall st,
   ex_reduce_teq_tm_1 / st ==>* tbool false / st.
 Proof.
   unfold ex_reduce_teq_tm_1. intros. repeat reduce. Qed.
 
-Definition ex_reduce_teq_tm_2 := ((
-    tvoid \== tvoid
-  )%oo).
+Definition ex_reduce_teq_tm_2 := tvoid \== tvoid.
 Example ex_reduce_teq_2:
   forall st,
   ex_reduce_teq_tm_2 / st ==>* tbool true / st.
 Proof.
   unfold ex_reduce_teq_tm_2. intros. repeat reduce. Qed.
 
-Definition ex_reduce_teq_tm_3 := ((
-    tnat 0 \== tnat 0
-  )%oo).
+Definition ex_reduce_teq_tm_3 := tnat 0 \== tnat 0.
 Example ex_reduce_teq_3:
   forall st,
   ex_reduce_teq_tm_3 / st ==>* tbool true / st.
 Proof.
   unfold ex_reduce_teq_tm_3. intros. repeat reduce. Qed.
 
-Definition ex_reduce_teq_tm_4 := ((
-    tbool true \== tbool true
-  )%oo).
+Definition ex_reduce_teq_tm_4 := tbool true \== tbool true.
 Example ex_reduce_teq_4:
   forall st,
   ex_reduce_teq_tm_4 / st ==>* tbool true / st.
 Proof.
   unfold ex_reduce_teq_tm_4. intros. repeat reduce. Qed.
 
-Definition ex_reduce_teq_tm_5 := ((
-    tref 0 \== tref 0
-  )%oo).
+Definition ex_reduce_teq_tm_5 := tref 0 \== tref 0.
 Example ex_reduce_teq_5:
   forall st,
   ex_reduce_teq_tm_5 / st ==>* tbool true / st.
 Proof.
   unfold ex_reduce_teq_tm_5. intros. repeat reduce. Qed.
 
-Definition ex_reduce_teq_tm_6 := ((
-    trc (tbool true) tvoid \== trc (tbool true) tvoid
-  )%oo).
+Definition ex_reduce_teq_tm_6 := trc (tbool true) tvoid \== trc (tbool true) tvoid.
 Example ex_reduce_teq_6:
   forall st,
   ex_reduce_teq_tm_6 / st ==>* tbool true / st.
 Proof.
   unfold ex_reduce_teq_tm_6. intros. repeat reduce. Qed.
 
-Definition ex_reduce_teq_tm_7 := ((
-    tcl "Foo" tvoid \== tcl "Foo" tvoid
-  )%oo).
+Definition ex_reduce_teq_tm_7 := tcl "Foo" tvoid \== tcl "Foo" tvoid.
 Example ex_reduce_teq_7:
   forall st,
   ex_reduce_teq_tm_7 / st ==>* tbool true / st.
 Proof.
   unfold ex_reduce_teq_tm_7. intros. repeat reduce. Qed.
 
-Definition ex_reduce_tvar_tm := ((
-    tvar 0
-  )%oo).
+Definition ex_reduce_tvar_tm := tvar 0.
 Example ex_reduce_tvar:
   let st := write_sk_hd 0 (tbool true) (resize_sk_hd 1 init_state) in
   ex_reduce_tvar_tm / st ==>* tbool true / st.
 Proof.
   unfold ex_reduce_tvar_tm. repeat reduce. Qed.
 
-Definition ex_reduce_tassign_tm := ((
-    tvar 0 ::= tnat 1 \+ tnat 1
-  )%oo).
+Definition ex_reduce_tassign_tm := tvar 0 ::= tnat 1 \+ tnat 1.
 Example ex_reduce_tassign:
   let st := resize_sk_hd 1 init_state in
   let st' := write_sk_hd 0 (tnat 2) st in
@@ -155,10 +125,9 @@ Example ex_reduce_tassign:
 Proof.
   unfold ex_reduce_tassign_tm. repeat reduce. Qed.
 
-Definition ex_reduce_tseq_tm := ((
+Definition ex_reduce_tseq_tm :=
     tvar 0 ::= tnat 1 \+ tnat 1;
-    tnat 3 \+ tvar 0
-  )%oo).
+    tnat 3 \+ tvar 0.
 Example ex_reduce_tseq:
   let st := resize_sk_hd 1 init_state in
   let st' := write_sk_hd 0 (tnat 2) st in
@@ -166,7 +135,7 @@ Example ex_reduce_tseq:
 Proof.
   unfold ex_reduce_tseq_tm. repeat reduce. Qed.
 
-Definition ex_reduce_tif_tm := ((
+Definition ex_reduce_tif_tm :=
     \if !tbool true
     \then
       tnat 1
@@ -177,15 +146,14 @@ Definition ex_reduce_tif_tm := ((
       \else
         tnat 3
       \fi
-    \fi
-  )%oo).
+    \fi.
 Example ex_reduce_tif:
   forall st,
   ex_reduce_tif_tm / st ==>* tnat 2 / st.
 Proof.
   unfold ex_reduce_tif_tm. intros. repeat reduce. Qed.
 
-Definition ex_reduce_twhile_tm := (
+Definition ex_reduce_twhile_tm :=
   let x := tvar 1 in
   let y := tvar 2 in
   (
@@ -196,7 +164,7 @@ Definition ex_reduce_twhile_tm := (
       x ::= x \- tnat 1
     \done;
     y
-  )%oo).
+  ).
 Example ex_reduce_twhile:
   let st := write_sk_hd 1 (tnat 3) (resize_sk_hd 3 init_state) in
   let st' := write_sk_hd 1 (tnat 0) (write_sk_hd 2 (tnat 6) st) in
@@ -204,97 +172,81 @@ Example ex_reduce_twhile:
 Proof.
   unfold ex_reduce_twhile_tm. repeat reduce. Qed.
 
-Definition ex_reduce_trc_tm := list_to_rc (cons (tnat 1 \+ tnat 2)%oo (cons (tnat 3 \+ tnat 4)%oo nil)).
+Definition ex_reduce_trc_tm := list_to_rc (cons (tnat 1 \+ tnat 2) (cons (tnat 3 \+ tnat 4) nil)).
 Example ex_reduce_trc:
   forall st,
   ex_reduce_trc_tm / st ==>* list_to_rc (cons (tnat 3) (cons (tnat 7) nil)) / st.
 Proof.
   unfold ex_reduce_trc_tm. intros. simpl. repeat reduce. Qed.
 
-Definition ex_reduce_tcall_tm := ((
-    tcall "foo" (<(tnat 1 \+ tnat 1)>)
-  )%oo).
+Definition ex_reduce_tcall_tm := tcall "foo" (<(tnat 1 \+ tnat 1)>).
 Example ex_reduce_tcall:
   forall st,
   ex_reduce_tcall_tm / st ==>* treturn (texec "foo") / push_call (trc (tnat 2) tvoid) st.
 Proof.
   unfold ex_reduce_tcall_tm. intros. simpl. repeat reduce. Qed.
 
-Definition ex_reduce_treturn_tm := ((
-    treturn (tnat 1 \+ tnat 1)
-  )%oo).
+Definition ex_reduce_treturn_tm := treturn (tnat 1 \+ tnat 1).
 Example ex_reduce_treturn:
   forall st,
   ex_reduce_treturn_tm / st ==>* tnat 2 / pop_call st.
 Proof.
   unfold ex_reduce_treturn_tm. intros. repeat reduce. Qed.
 
-Definition ex_reduce_tcl_tm := ((
-    tcl "foo" (<(tnat 1 \+ tnat 1)>)
-  )%oo).
+Definition ex_reduce_tcl_tm := tcl "foo" (<(tnat 1 \+ tnat 1)>).
 Example ex_reduce_tcl:
   forall st,
   ex_reduce_tcl_tm / st ==>* tcl "foo" (trc (tnat 2) tvoid) / st.
 Proof.
   unfold ex_reduce_tcl_tm. intros. repeat reduce. Qed.
 
-Definition ex_reduce_tnew_tm := ((
-    tnew 2 "foo"
-  )%oo).
+Definition ex_reduce_tnew_tm := tnew 2 "foo".
 Example ex_reduce_tnew:
-  ex_reduce_tnew_tm / init_state ==>* tref 1 / alloc_sr (tcl "foo" (<(tvoid, tvoid)>))%oo init_state.
+  ex_reduce_tnew_tm / init_state ==>* tref 1 / alloc_sr (tcl "foo" (<(tvoid, tvoid)>)) init_state.
 Proof.
   unfold ex_reduce_tnew_tm. repeat reduce. Qed.
 
-Definition ex_reduce_tfield_r_tm := ((
-    (treturn (tref 1))@2
-  )%oo).
+Definition ex_reduce_tfield_r_tm := (treturn (tref 1))@2.
 Example ex_reduce_tfield_r:
-  let st := push_call tvoid (alloc_sr (tcl "foo" (<(tvoid, tnat 1, tnat 2)>))%oo init_state) in
+  let st := push_call tvoid (alloc_sr (tcl "foo" (<(tvoid, tnat 1, tnat 2)>)) init_state) in
   let st' := pop_call st in
   ex_reduce_tfield_r_tm / st ==>* tnat 2 / st'.
 Proof.
   unfold ex_reduce_tfield_r_tm. repeat reduce. Qed.
 
-Definition ex_reduce_tfield_w_tm := ((
-    (treturn (tref 1)) <@ 1 <- (tnat 1 \+ tnat 1)
-  )%oo).
+Definition ex_reduce_tfield_w_tm := (treturn (tref 1)) <@ 1 <- (tnat 1 \+ tnat 1).
 Example ex_reduce_tfield_w:
-  let st := push_call tvoid (alloc_sr (tcl "foo" (<(tvoid, tvoid)>))%oo init_state) in
-  let st' := write_sr 1 (tcl "foo" (<(tvoid, tnat 2)>))%oo (pop_call st) in
+  let st := push_call tvoid (alloc_sr (tcl "foo" (<(tvoid, tvoid)>)) init_state) in
+  let st' := write_sr 1 (tcl "foo" (<(tvoid, tnat 2)>)) (pop_call st) in
   ex_reduce_tfield_w_tm / st ==>* tvoid / st'.
 Proof.
   unfold ex_reduce_tfield_w_tm. repeat reduce. Qed.
 
-Definition ex_reduce_tvnew_tm := ((
-    tvnew 2 "foo"
-  )%oo).
+Definition ex_reduce_tvnew_tm := tvnew 2 "foo".
 Example ex_reduce_tvnew:
   forall st,
-  ex_reduce_tvnew_tm / st ==>* (tcl "foo" (<(tvoid, tvoid)>))%oo / st.
+  ex_reduce_tvnew_tm / st ==>* (tcl "foo" (<(tvoid, tvoid)>)) / st.
 Proof.
   unfold ex_reduce_tvnew_tm. intros. repeat reduce. Qed.
 
-Definition ex_reduce_tvfield_r_tm := ((
-    tcl "foo" (<(tvoid, tnat 1, tnat 1 \+ tnat 1)>)?@2
-  )%oo).
+Definition ex_reduce_tvfield_r_tm := tcl "foo" (<(tvoid, tnat 1, tnat 1 \+ tnat 1)>)?@2.
 Example ex_reduce_tvfield_r:
   forall st,
   ex_reduce_tvfield_r_tm / st ==>* tnat 2 / st.
 Proof.
   unfold ex_reduce_tvfield_r_tm. intros. repeat reduce. Qed.
 
-Definition ex_reduce_tvfield_w_tm := ((
-    (tvar 0) <?@ 1 <- (tnat 1 \+ tnat 1)
-  )%oo).
+Definition ex_reduce_tvfield_w_tm := (tvar 0) <?@ 1 <- (tnat 1 \+ tnat 1).
 Example ex_reduce_tvfield_w:
-  let st := write_sk_hd 0 (tcl "foo" (<(tvoid, tvoid)>))%oo (resize_sk_hd 1 init_state) in
-  let st' := write_sk_hd 0 (tcl "foo" (<(tvoid, tnat 2)>))%oo st in
+  let st := write_sk_hd 0 (tcl "foo" (<(tvoid, tvoid)>)) (resize_sk_hd 1 init_state) in
+  let st' := write_sk_hd 0 (tcl "foo" (<(tvoid, tnat 2)>)) st in
   ex_reduce_tvfield_w_tm / st ==>* tvoid / st'.
 Proof.
   unfold ex_reduce_tvfield_w_tm. repeat reduce. Qed.
 
 End Examples.
+
+Open Scope oo_scope.
 
 Definition main : tm := (
   let x := tvar 1 in
@@ -308,5 +260,5 @@ Definition main : tm := (
       x ::= x \- tnat 1
     \done;
     y
-  )%oo).
+  )).
 
